theories/interop/embed_wp.v
@@ -19,14 +19,14 @@ Implicit Types v : val.
 Implicit Types T : string -d> list val -d> (val -d> iPropO Σ) -d> iPropO Σ.
 
 Global Program Instance embed_mlangGS :
-  mlanguage.weakestpre.mlangGS hlc val Σ (embed_lang Λ)
+  mlanguage.weakestpre.mlangGS hlc val Σ (lang_to_mlang Λ)
 := {
   state_interp := (λ σ, ∃ n, language.weakestpre.state_interp σ n)%I;
   at_boundary := True%I;
 }.
 
 Global Program Instance embed_linkableGS :
-  linkableGS (embed_lang Λ) (λ σ, ∃ n, language.weakestpre.state_interp σ n)%I
+  linkableGS (lang_to_mlang Λ) (λ σ, ∃ n, language.weakestpre.state_interp σ n)%I
 := {
   private_state_interp := (λ _, True)%I;
 }.
@@ -36,24 +36,28 @@ Next Obligation.
 Qed.
 Next Obligation. simpl. iIntros (σ) "_ Hσ". iPureIntro. exists σ, (). constructor. Qed.
 
-Definition lang_prog_environ p T : language.weakestpre.prog_environ Λ :=
-   language.weakestpre.Build_prog_environ hlc _ _ _ _ p T.
-Definition mlang_prog_environ p T : mlanguage.weakestpre.prog_environ (embed_lang Λ) :=
-   mlanguage.weakestpre.Build_prog_environ hlc _ _ _ _ _ p T.
+Local Canonical Structure embed_mlang : mlanguage val := lang_to_mlang Λ.
 
-Lemma wp_embed e p T E Φ :
-  ⊢ WP e @ lang_prog_environ p T ; E {{ Φ }} -∗ WP e @ mlang_prog_environ p T ; E {{ Φ }}.
+Definition penv_to_mlang (pe : language.weakestpre.prog_environ Λ Σ) :
+  mlanguage.weakestpre.prog_environ (lang_to_mlang Λ) Σ
+:=
+  {| penv_prog := pe.(language.weakestpre.penv_prog);
+     penv_proto := pe.(language.weakestpre.penv_proto) |}.
+
+Lemma wp_embed (e : Λ.(language.expr)) pe E Φ :
+  ⊢ WP e @ pe; E {{ Φ }} -∗ WP e @ (penv_to_mlang pe); E {{ Φ }}.
 Proof using.
-  iStartProof. iLöb as "IH" forall (e).
-  rewrite {1} @language.weakestpre.wp_unfold /language.weakestpre.wp_pre.
-  rewrite {1} wp_unfold /wp_pre.
+  iStartProof. iLöb as "IH" forall (e). destruct pe as [p T].
+  rewrite {1} @language.weakestpre.wp_unfold /language.weakestpre.wp_pre. simpl.
+  rewrite {1} wp_unfold /mlanguage.weakestpre.wp_pre.
   iIntros "H" (σ) "(%n & Hσ)". iMod ("H" $! σ n with "Hσ") as "[(%x & %H1 & Hσ & H)|[(%s' & %vv & %K' & %H1 & %H2 & H3)|(%Hred & H3)]]".
   - iLeft. iModIntro. iExists x. iFrame. iSplitR; first done. iExists n. iFrame.
   - iRight. iLeft. iMod "H3" as "(%Ξ & Hσ & HT & Hr)". iExists s', vv, K'. iModIntro.
     iSplitR; first done. iSplitR; first done. iSplitR; first done. iSplitL "Hσ"; first by iExists n.
     iExists Ξ. iFrame. iNext. iIntros (v) "[Hv _]". iApply "IH". by iApply "Hr".
   - iRight. iRight. iModIntro. iSplitR.
-    { iPureIntro. destruct Hred as (e' & σ' & H'). eexists (fun '(e2,σ2) => e2 = e' ∧ σ2 = σ'). inversion H'; subst. econstructor. eexists; split; first done. econstructor; first done. intros ? ? ( <- & <- ); done. }
+    { iPureIntro. destruct Hred as (e' & σ' & H'). eexists (fun '(e2,σ2) => e2 = e' ∧ σ2 = σ'). inversion H'; subst. econstructor. eexists; split; first done.
+      econstructor; first done. intros ? ? ( <- & <- ); done. }
     iIntros (X Hstep). inversion Hstep as (K & e' & -> & Hx). inversion Hx; subst.
     unshelve iMod ("H3" $! σ2 _ (Prim_step _ K _ _ _ _ _ _ _ _ _ H3)) as "H3". 1-2:done.
     do 2 iModIntro. iMod "H3" as "(Hσ & Hwp)". iModIntro. iExists _, _. iSplitR; first (iPureIntro; apply H5; repeat split).
@@ -61,3 +65,5 @@ Proof using.
 Qed.
 
 End Embed_logic.
+
+Global Arguments penv_to_mlang {_ _ _} _.
