theories/mlanguage/lifting.v
@@ -8,7 +8,7 @@ From iris.prelude Require Import options.
 Section lifting.
 Context `{!invGS_gen hlc Σ, !mlangGS hlc val Σ Λ}.
 Implicit Types prog : mixin_prog (func Λ).
-Implicit Types s : prog_environ Λ.
+Implicit Types pe : prog_environ Λ Σ.
 Implicit Types v : val.
 Implicit Types e : expr Λ.
 Implicit Types σ : state Λ.
@@ -16,14 +16,14 @@ Implicit Types P Q : iProp Σ.
 Implicit Types Φ : val → iProp Σ.
 Implicit Types X : expr Λ * state Λ → Prop.
 
-Lemma wp_lift_step_fupd s E Φ e1 :
+Lemma wp_lift_step_fupd pe E Φ e1 :
   to_val e1 = None →
   (∀ σ1, state_interp σ1 ={E}=∗
-    ⌜reducible (prog s) e1 σ1⌝ ∗
-    ∀ X, ⌜prim_step (prog s) (e1, σ1) X⌝ ={E}▷=∗^(1) |={E}=>
+    ⌜reducible (penv_prog pe) e1 σ1⌝ ∗
+    ∀ X, ⌜prim_step (penv_prog pe) (e1, σ1) X⌝ ={E}▷=∗^(1) |={E}=>
       ∃ e2 σ2,
-        ⌜X (e2, σ2)⌝ ∗ state_interp σ2 ∗ WP e2 @ s; E {{ Φ }})
-  ⊢ WP e1 @ s; E {{ Φ }}.
+        ⌜X (e2, σ2)⌝ ∗ state_interp σ2 ∗ WP e2 @ pe; E {{ Φ }})
+  ⊢ WP e1 @ pe; E {{ Φ }}.
 Proof. intros H. rewrite wp_unfold /wp_pre.
   iIntros "H %σ Hσ". iMod ("H" $! σ with "Hσ") as "[H1 H2]". iModIntro. do 2 iRight.
   iFrame. iIntros (X Hstep). iMod ("H2" $! X Hstep) as "H2". do 2 iModIntro.
@@ -34,17 +34,17 @@ Qed.
 (** Derived lifting lemmas. *)
 
 
-Lemma wp_lift_atomic_step {s E Φ} e1 :
+Lemma wp_lift_atomic_step {pe E Φ} e1 :
   to_val e1 = None →
   (∀ σ1, state_interp σ1 ={E}=∗
-    ⌜reducible (prog s) e1 σ1⌝ ∗
-    ▷ ∀ X, ⌜prim_step (prog s) (e1, σ1) X⌝ ={E}=∗
+    ⌜reducible (penv_prog pe) e1 σ1⌝ ∗
+    ▷ ∀ X, ⌜prim_step (penv_prog pe) (e1, σ1) X⌝ ={E}=∗
       ∃ e2 σ2, ⌜X (e2, σ2)⌝ ∗
         state_interp σ2 ∗ from_option Φ False (to_val e2))
-  ⊢ WP e1 @ s; E {{ Φ }}.
+  ⊢ WP e1 @ pe; E {{ Φ }}.
 Proof.
   iIntros (?) "H".
-  iApply (wp_lift_step_fupd s E _ e1)=>//; iIntros (σ1) "Hσ1".
+  iApply (wp_lift_step_fupd pe E _ e1)=>//; iIntros (σ1) "Hσ1".
   iMod ("H" $! σ1 with "Hσ1") as "[$ H]". iModIntro.
   iIntros (X Hstep). do 3 iModIntro.
   iMod ("H" $! X Hstep) as (e' σ' HX) "[? ?]". iModIntro.
@@ -53,17 +53,17 @@ Proof.
   by iApply wp_value.
 Qed.
 
-Lemma wp_lift_atomic_head_step {s E Φ} e1 :
+Lemma wp_lift_atomic_head_step {pe E Φ} e1 :
   to_val e1 = None →
   (∀ σ1, state_interp σ1 ={E}=∗
-    ⌜head_reducible (prog s) e1 σ1⌝ ∗
-    ▷ ∀ X, ⌜head_step (prog s) (e1, σ1) X⌝ ={E}=∗
+    ⌜head_reducible (penv_prog pe) e1 σ1⌝ ∗
+    ▷ ∀ X, ⌜head_step (penv_prog pe) (e1, σ1) X⌝ ={E}=∗
       ∃ e2 σ2, ⌜X (e2, σ2)⌝ ∗
         state_interp σ2 ∗ from_option Φ False (to_val e2))
-  ⊢ WP e1 @ s; E {{ Φ }}.
+  ⊢ WP e1 @ pe; E {{ Φ }}.
 Proof.
   iIntros (?) "H".
-  iApply (wp_lift_step_fupd s E _ e1)=>//; iIntros (σ1) "Hσ1".
+  iApply (wp_lift_step_fupd pe E _ e1)=>//; iIntros (σ1) "Hσ1".
   iMod ("H" $! σ1 with "Hσ1") as "[%HH H]". iModIntro. iSplitR; first (iPureIntro; by eapply head_prim_reducible).
   iIntros (X Hstep%head_reducible_prim_step). 2:easy. do 3 iModIntro.
   iMod ("H" $! X Hstep) as (e' σ' HX) "[H1 H2]". iModIntro.
@@ -72,15 +72,15 @@ Proof.
   by iApply wp_value.
 Qed.
 
-Lemma wp_lift_pure_det_step `{!Inhabited (state Λ)} {s E Φ} e1 e2 :
-  (∀ σ1, reducible (prog s) e1 σ1) →
+Lemma wp_lift_pure_det_step `{!Inhabited (state Λ)} {pe E Φ} e1 e2 :
+  (∀ σ1, reducible (penv_prog pe) e1 σ1) →
   (∀ σ1 X,
-    prim_step (prog s) (e1, σ1) X →
+    prim_step (penv_prog pe) (e1, σ1) X →
     X (e2, σ1)) →
-  (|={E}[E]▷=> WP e2 @ s; E {{ Φ }}) ⊢ WP e1 @ s; E {{ Φ }}.
+  (|={E}[E]▷=> WP e2 @ pe; E {{ Φ }}) ⊢ WP e1 @ pe; E {{ Φ }}.
 Proof.
   iIntros (Hsafe Hstep) "H". iApply wp_lift_step_fupd.
-  { specialize (Hsafe inhabitant). destruct s; eauto using reducible_not_val. }
+  { specialize (Hsafe inhabitant). destruct pe; eauto using reducible_not_val. }
   iIntros (σ1) "Hσ". iMod "H". iModIntro.
   iSplitR; first (iPureIntro; apply Hsafe).
   iIntros (X Hstep'). do 3 iModIntro. iMod "H".
@@ -89,24 +89,24 @@ Proof.
   iFrame.
 Qed.
 
-Lemma wp_pure_step_fupd `{!Inhabited (state Λ)} s E e1 e2 φ n Φ :
-  PureExec φ n (prog s) e1 e2 →
+Lemma wp_pure_step_fupd `{!Inhabited (state Λ)} pe E e1 e2 φ n Φ :
+  PureExec φ n (penv_prog pe) e1 e2 →
   φ →
-  (|={E}[E]▷=>^n WP e2 @ s; E {{ Φ }}) ⊢ WP e1 @ s; E {{ Φ }}.
+  (|={E}[E]▷=>^n WP e2 @ pe; E {{ Φ }}) ⊢ WP e1 @ pe; E {{ Φ }}.
 Proof.
   iIntros (Hexec Hφ) "Hwp". specialize (Hexec Hφ).
   iInduction Hexec as [e|n e1 e2 e3 [Hsafe ?]] "IH"; simpl.
   { iMod lc_zero as "Hz". by iApply "Hwp". }
   iApply wp_lift_pure_det_step.
-  - intros σ. specialize (Hsafe σ). destruct s; eauto using reducible_not_val.
+  - intros σ. specialize (Hsafe σ). destruct pe; eauto using reducible_not_val.
   - intros. eapply pure_step_det; eauto.
   - iApply (step_fupd_wand with "Hwp"). iApply "IH".
 Qed.
 
-Lemma wp_pure_step_later `{!Inhabited (state Λ)} s E e1 e2 φ n Φ :
-  PureExec φ n (prog s) e1 e2 →
+Lemma wp_pure_step_later `{!Inhabited (state Λ)} pe E e1 e2 φ n Φ :
+  PureExec φ n (penv_prog pe) e1 e2 →
   φ →
-  ▷^n (WP e2 @ s; E {{ Φ }}) ⊢ WP e1 @ s; E {{ Φ }}.
+  ▷^n (WP e2 @ pe; E {{ Φ }}) ⊢ WP e1 @ pe; E {{ Φ }}.
 Proof.
   intros Hexec ?. rewrite -wp_pure_step_fupd //. clear Hexec.
   enough (∀ P, ▷^n P -∗ |={E}▷=>^n P) as Hwp by apply Hwp. iIntros (?).
